

$$b. \quad -(k(x)u')' + b(x)u' + c(x)u = f(x) \quad x \in \Omega = (\alpha, \beta) \\ u(\alpha) = u(\beta) = 0$$

$$\text{Let } v \in H_0^1(\Omega)$$

$$\int_{\Omega} -(k(x)u')' v(x) + b(x)u' v(x) + c(x)u v(x) d\Omega = \int_{\Omega} f(x)v(x) d\Omega$$

$$\int_{\Omega} -(k(x)u')' v(x) d\Omega = \int_{\partial\Omega} (k(x)u') \cdot \hat{n} v ds + \int_{\Omega} (k(x)u') v'(x) d\Omega$$

$$\text{Let } w(x) \text{ be the representation of } u \text{ in } \Omega \\ \int_{\Omega} k(x)w'(x)v'(x) + b(x)w'(x)v(x) + c(x)w(x)v(x) d\Omega = \int_{\Omega} f(x)v(x) d\Omega \\ B(w, v) = F(v)$$

bi. Since $0 < k_m \leq k(x) \leq K_m < \infty \quad \forall x \in \Omega$, we know k is bdd and positive.

$$|B(w, v)| = \left| \int_{\Omega} k(x)w'(x)v'(x) + b(x)w'(x)v(x) + c(x)w(x)v(x) d\Omega \right| \\ \leq \left| \int_{\Omega} k(x)w'(x)v'(x) d\Omega \right| + \left| \int_{\Omega} b(x)w'(x)v(x) d\Omega \right| + \left| \int_{\Omega} c(x)w(x)v(x) d\Omega \right| \\ \leq k_m \left(\int_{\Omega} w'^2 d\Omega \right)^{1/2} \left(\int_{\Omega} v'^2 d\Omega \right)^{1/2} + \|b\|_{\infty} \left(\int_{\Omega} w'^2 d\Omega \right)^{1/2} \left(\int_{\Omega} |v|^2 d\Omega \right)^{1/2} \\ + \|c\|_{\infty} \left(\int_{\Omega} w^2 d\Omega \right)^{1/2} \left(\int_{\Omega} |v|^2 d\Omega \right)^{1/2} \\ \leq k_m \|w\|_{H^1} \|v\|_{H^1} + \|b\|_{\infty} \|w\|_{H^1} \|v\|_{H^1} + \|c\|_{\infty} \|w\|_{H^1} \|v\|_{H^1} \\ = (k_m + \|b\|_{\infty} + \|c\|_{\infty}) \|w\|_{H^1} \|v\|_{H^1}$$

Thus b & c need to be in L^{∞}

$$\text{bii. } |B(w, w)| = \left| \int_{\Omega} k(x)(w')^2 + b w' w + c(w)^2 d\Omega \right|$$

$$= \int_{\Omega} k(x)(w')^2 d\Omega + \int_{\Omega} b(w^2)' d\Omega + \int_{\Omega} c(w)^2 d\Omega$$

$$\frac{1}{2} \int_{\Omega} b(w^2)' d\Omega = \frac{1}{2} \int_{\partial\Omega} b \cdot \hat{n} (w^2) ds - \frac{1}{2} \int_{\Omega} b' w^2 d\Omega$$

$$\geq \left| k_m \|w'\|_2^2 - \frac{1}{2} \int_{\Omega} b' w^2 d\Omega + \int_{\Omega} c w^2 d\Omega \right|$$

$$= \left| k_m \|w'\|_2^2 + \int_{\Omega} (c - \frac{1}{2} b') w^2 d\Omega \right|$$

$$\geq (k_m + C_{PF}) \|w\|_{H^1}^2 \quad \text{given } c - \frac{1}{2} b' \geq 0 \quad \forall x \in \Omega \quad \text{Since } w(\alpha) = w(\beta) = 0 \\ \geq C_E (k_m + C_{PF}) \|w\|_{H^1}^2 \quad \text{since equivalent norms}$$

Thus $c - \frac{1}{2} b' \geq 0$ is the restriction so that B is coercive

$$\begin{aligned}
 \text{1c. } f \in L^2 \quad |F(v)| &= \left| \int_{\Omega} f v \, d\Omega \right| \\
 &\leq \left(\int_{\Omega} |f|^2 \, d\Omega \right)^{1/2} \left(\int_{\Omega} |v|^2 \, d\Omega \right)^{1/2} \\
 &= \|f\|_2 \|v\|_2 \\
 &\leq \|f\|_2 \|v\|_{H^1}
 \end{aligned}$$

Since $f \in L^2$, $\|f\|_2 < \infty$ Thus $F(v)$ is bdd

$$\|F\| = \sup_{\|v\|_{H^1}=1} |F(v)| \leq \sup_{\|v\|_{H^1}=1} \|f\|_2 \|v\|_{H^1} = \|f\|_2 < \infty$$

$\therefore F$ is a bdd linear functional

1d. Let $v_1, v_2, w_1, w_2 \in H_0^1(\Omega)$ and $\delta \in \mathbb{R}$

$$\begin{aligned}
 F(\delta v_1 + v_2) &= \int_{\Omega} f(\delta v_1 + v_2) \, d\Omega = \delta \int_{\Omega} f v_1 \, d\Omega + \int_{\Omega} f v_2 \, d\Omega \\
 &= \delta F(v_1) + F(v_2)
 \end{aligned}$$

$$\begin{aligned}
 B(\delta w_1 + w_2, v_1) &= \int_{\Omega} k(\delta w_1 + w_2)' v_1' + b(\delta w_1 + w_2)' v_1 + c(\delta w_1 + w_2) v_1 \, d\Omega \\
 &= \delta \int_{\Omega} k w_1' v_1' + b w_1' v_1 + c w_1 v_1 \, d\Omega + \int_{\Omega} k w_2' v_1' + b w_2' v_1 + c w_2 v_1 \, d\Omega \\
 &= \delta B(w_1, v_1) + B(w_2, v_1)
 \end{aligned}$$

$$\begin{aligned}
 B(w_1, \delta v_1 + v_2) &= \int_{\Omega} k w_1' (\delta v_1 + v_2)' + b w_1' (\delta v_1 + v_2) + c w_1 (\delta v_1 + v_2) \, d\Omega \\
 &= \delta \int_{\Omega} k w_1' v_1' + b w_1' v_1 + c w_1 v_1 \, d\Omega + \int_{\Omega} k w_1' v_2' + b w_1' v_2 + c w_1 v_2 \, d\Omega \\
 &= \delta B(w_1, v_1) + B(w_1, v_2)
 \end{aligned}$$

Thus $B(\cdot, \cdot)$ is coercive, bilinear, and bdd
and $F(\cdot)$ is a bdd linear functional, therefore
 $\exists! u \in H_0^1 \ni B(u, v) = F(v) \quad \forall v \in H_0^1$

1cont. As the span of L.I. elements of $H_0^1(\Omega)$,
 $\mathcal{S}_N \subseteq H_0^1(\Omega)$.

Note $B|_{\mathcal{S}_N}$ and $F|_{\mathcal{S}_N}$ still fit the requirements for the Lax-Milgram theorem since the domain does not change bddness, coercivity, or (bi)linearity of B or F

cont. cont \therefore by Lax-Milgram $\exists! u_h \in S_N \ni$
 $B(u_h, v_h) = F(v_h) \quad \forall v_h \in S_N$

It follows by Cea's lemma that

$$\|e\|_{H_0} = \|u - u_h\|_{H_1} \leq \left(1 + \frac{c_1}{c_2}\right) \inf_{w_h \in S_N} \|u - w_h\|_{H_0}$$